add a generic Hybrid proof.

theories/Means.ec
@@ -26,7 +26,7 @@ theory Mean.
     }
   }.
 
-  lemma prCond (A<:Worker{Rand}) &m (v:input) 
+  lemma prCond (A<:Worker) &m (v:input) 
                (ev:input -> glob A -> output -> bool) : 
       Pr[Rand(A).randAndWork() @ &m :
            ev v (glob A) (snd res) /\ v = fst res] = 
@@ -46,13 +46,13 @@ theory Mean.
     conseq* (_: _ ==> false) => //.
   qed.
 
-  lemma introOrs (A<:Worker{Rand}) &m (ev:input -> glob A -> output -> bool) :
+  lemma introOrs (A<:Worker) &m (ev:input -> glob A -> output -> bool) :
      Finite.finite (create (support d)) =>
      let sup = Finite.toFSet (create (support d)) in
      Pr[Rand(A).randAndWork() @ &m : ev (fst res) (glob A) (snd res)] =
      Pr[Rand(A).randAndWork() @ &m : 
        cpOrs (img (lambda v r, ev v (glob A) (snd r) /\ v = fst r) sup) res].
-  proof.
+  proof strict.
     intros Fsup sup.
     equiv_deno (_: ={glob A} ==> ={glob A, res} /\ in_supp (fst res{1}) d)=> //.
       by fun; call (_: true); rnd.
@@ -67,14 +67,14 @@ theory Mean.
     by rewrite img_def => /= [ [v [<- /= Hm] [H1 <- ]]].
   save.
 
-  lemma Mean (A<:Worker {Rand}) &m (ev:input -> glob A -> output -> bool): 
+  lemma Mean (A<:Worker) &m (ev:input -> glob A -> output -> bool): 
      Finite.finite (create (support d)) =>
      let sup = Finite.toFSet (create (support d)) in
      Pr[Rand(A).randAndWork()@ &m: ev (fst res) (glob A) (snd res)] =
        Mrplus.sum
         (lambda (v:input), mu_x d v * Pr[A.work(v)@ &m:ev v (glob A) res]) 
         sup.
-  proof.
+  proof strict.
     intros Fsup; rewrite /=.
     cut := introOrs A &m ev _ => //= ->.
     elimT set_ind (Finite.toFSet (create (support d))).
@@ -101,4 +101,424 @@ theory Mean.
     by rewrite Hrec (prCond A &m x ev).
   qed.
 
-end Means.
+  lemma Mean_uni (A<:Worker) &m (ev:input -> glob A -> output -> bool) r: 
+     (forall x, in_supp x d => mu_x d x = r) =>
+     Finite.finite (create (support d)) =>
+     let sup = Finite.toFSet (create (support d)) in
+     Pr[Rand(A).randAndWork()@ &m: ev (fst res) (glob A) (snd res)] =
+       r * Mrplus.sum (lambda (v:input), Pr[A.work(v)@ &m:ev v (glob A) res]) sup.
+  proof.
+    intros Hd Hfin /=.
+    cut := Mean A &m ev => /= -> //.
+    cut := Mrplus.sum_comp (( * ) r) (lambda (v:input), Pr[A.work(v)@ &m:ev v (glob A) res]) => /= <-.
+      by intros x y;ringeq.
+    apply Mrplus.sum_eq => /= x.
+    by rewrite Finite.mem_toFSet // mem_create /support => Hin;rewrite Hd.
+  qed.
+   
+end Mean.
+
+theory LR.
+
+  clone import Mean as M with
+    type input <- bool,
+    type output <- bool,
+    op d <- {0,1}.
+
+  lemma Sample_LR (A<:Worker) &m:
+    Pr[A.work(false) @ &m : true] = 1%r =>
+    Pr[Rand(A).randAndWork() @ &m : fst res = snd res] - 1%r/2%r = 
+      1%r/2%r*(Pr[A.work(true) @ &m : res] - Pr[A.work(false) @ &m : res]).
+  proof strict.
+    intros Hloss.
+    pose ev := lambda (b:bool) (gA:glob A) (b':bool), b = b'.
+    cut -> : Pr[Rand(A).randAndWork() @ &m : fst res = snd res] =
+             Pr[Rand(A).randAndWork() @ &m : ev (fst res) (glob A) (snd res)] by trivial.
+    cut Hcr: forall x, 
+               mem x (create (support {0,1})) <=>
+               mem x (add true (add false (FSet.empty)%FSet)) by smt.
+    cut Hf : Finite.finite (create (support {0,1})).
+      by exists (FSet.add true (FSet.add false FSet.empty)) => x;apply Hcr.
+    cut := Mean A &m ev => /= -> //.
+    cut -> : 
+      Finite.toFSet (create (support {0,1})) = (FSet.add true (FSet.add false FSet.empty)).
+      by apply FSet.set_ext => x; rewrite Finite.mem_toFSet //;apply Hcr.
+    rewrite Mrplus.sum_add;first smt.
+    rewrite Mrplus.sum_add;first smt.
+    rewrite Mrplus.sum_empty /= !Bool.Dbool.mu_x_def;simplify ev.
+    cut Hd: 2%r <> zero by smt.
+    cut -> : Pr[A.work(true) @ &m : true = res] = Pr[A.work(true) @ &m : res].
+      by rewrite Pr mu_eq;smt.
+    cut -> : Pr[A.work(false) @ &m : false = res] = Pr[A.work(false) @ &m : !res].
+      by rewrite Pr mu_eq;smt.       
+    rewrite Pr mu_not.
+    by rewrite Hloss;fieldeq.
+  save.
+
+end LR.
+
+theory Hybrid.
+  type input.
+  type output.
+  type leaks.
+
+  module type Enc = { 
+    fun init () : unit { * }
+    fun leaks () : leaks  
+    fun enc (m:input) : output
+  }.
+
+  module type AEnc = {
+    fun leaks () : leaks  
+    fun enc (m:input) : output
+  }.
+
+  module type LR = { 
+    fun lr(m0 m1:input) : output
+  }.
+
+  module type Mk_LR(E:AEnc) = {
+    fun lr(m0 m1:input) : output
+  }.
+    
+(*  module L(E:Enc) = {
+    fun lr(m0 m1:input) : output = {
+      var r : output;
+      r = E.enc(m0);
+      return r;
+    }
+  }.
+
+  module R(E:Enc) = {
+    fun lr(m0 m1:input) : output = {
+      var r : output;
+      r = E.enc(m1);
+      return r;
+    }
+  }. 
+*)
+
+  module type Adv(E:AEnc, LR:LR) = {
+    fun run () : bool
+  }.
+
+  import Int.
+
+  module N (E:Enc, LR:LR, A:Adv) = {
+    var c:int
+
+    module LRc = {
+      fun lr(m0 m1:input) : output = {
+        var r : output;
+        c = c + 1;
+        r = LR.lr(m0, m1);
+        return r;
+      }
+    }
+
+    module A = A(E,LRc)
+
+    fun main () : bool = {
+      var b' : bool;
+      c = 0;        
+      E.init();
+      b' = A.run();
+      return b';
+    }
+  }.
+
+  op q : int.
+
+  clone import Mean as M with
+    type input <- int,
+    type output <- bool,
+    op d <- [0..q-1].
+
+  module LRB (L: LR, R: LR, LR0:LR) = {
+    var l, l0 : int  
+    fun lr(m0 m1:input):output = {
+      var r : output;
+      if (l0 < l) r = L.lr(m0,m1);
+      else { 
+        if (l0 = l) r = LR0.lr(m0,m1);
+        else r = R.lr(m0,m1);
+      }
+      l = l + 1;
+      return r;
+    }
+  }.
+ 
+  module B(A:Adv, L:LR, R:LR, E:AEnc, LR0:LR) = {
+    module LR = LRB(L,R,LR0)
+    module A = A(E,LR)
+    fun run():bool = {
+      var b':bool;
+      LRB.l0 = $[0..q-1];
+      LRB.l  = 0;
+      b' = A.run();
+      return b' && LRB.l <= q;
+    }
+  }.
+
+  section.
+
+  declare module E    : Enc   {N,LRB}.
+  declare module ML   : Mk_LR {N,LRB,E}.
+  declare module MR   : Mk_LR {N,LRB,E,ML}.  
+  declare module A    : Adv   {N,LRB,E,ML,MR}.
+  
+  local module L   = ML(E).
+  local module R   = MR(E).
+  local module LRBL = LRB(L,R,L).
+  local module LRBR = LRB(L,R,R).
+
+  local module BA  = B(A, L, R).
+  local module NLB = N(E,L,BA).
+  local module NRB = N(E,R,BA).  
+
+
+  local module W (LR0:LR) = {
+    module LR = LRB(L,R,LR0)
+    module A = A(E,LR)
+    fun work(x:int) : bool = {
+      var b':bool;
+      LRB.l = 0; LRB.l0 = x;
+      E.init();
+      b' = A.run();
+      return b' && LRB.l <= q;
+    }
+  }.
+
+  local equiv Einit : E.init ~ E.init : true ==> ={glob E}.
+  proof strict.
+    by fun true.
+  qed.
+
+  local equiv Eleaks : E.leaks ~ E.leaks : ={glob E} ==> ={res,glob E}.
+  proof strict.
+    by fun true.   
+  qed.
+
+  local equiv Eenc : E.enc ~ E.enc : ={m,glob E} ==> ={res,glob E}.
+  proof strict.
+    by fun true.   
+  qed.
+
+  local equiv Eml : ML(E).lr ~ ML(E).lr : ={m0,m1,glob ML, glob E} ==> ={res, glob ML, glob E}.
+  proof strict.
+    fun (={glob E})=> //;[apply Eleaks | apply Eenc].
+  qed.
+
+  local equiv Emr : MR(E).lr ~ MR(E).lr : ={m0,m1,glob MR, glob E} ==> ={res, glob MR, glob E}.
+  proof strict.
+    fun (={glob E})=> //;[apply Eleaks | apply Eenc].
+  qed.
+ 
+  local lemma NWL &m :
+    Pr[N(E,L,BA).main() @ &m : res /\ N.c <= 1] = 
+    Pr[Rand(W(L)).randAndWork() @ &m : snd res].
+  proof strict.
+    equiv_deno (_ : ={glob A, glob ML, glob MR} ==> 
+                    res{1} = snd res{2} /\ N.c{1} <= 1) => //.
+    fun. 
+    inline{1} N(E, ML(E), B(A, ML(E), MR(E))).A.run.
+    inline{2} W(ML(E)).work;wp.
+    call (_: ={glob ML, glob MR, glob E, glob LRB} /\ N.c{1} = (LRB.l0{1} < LRB.l{1}) ? 1 : 0).
+      fun;wp.
+      if => //.
+        by call Eml;skip;progress => //; smt.
+      if => //.
+        inline{1} N(E, ML(E), B(A, ML(E), MR(E))).LRc.lr;wp.
+        by call Eml;wp;skip;progress => //;smt.
+      by call Emr;skip;progress => //; smt.
+      by conseq * Eleaks.
+      by conseq * Eenc.
+    swap{1} 2 2.
+    by call Einit;wp;rnd;wp;skip;progress => //;smt.
+  qed.
+
+  local lemma NWR &m :
+    Pr[N(E,R,BA).main() @ &m : res /\ N.c <= 1] = 
+    Pr[Rand(W(R)).randAndWork() @ &m : snd res].
+  proof strict.
+    equiv_deno (_ : ={glob A, glob ML, glob MR} ==> 
+                    res{1} = snd res{2} /\ N.c{1} <= 1) => //.
+    fun. 
+    inline{1} N(E, MR(E), B(A, ML(E), MR(E))).A.run.
+    inline{2} W(MR(E)).work;wp.
+    call (_: ={glob ML, glob MR, glob E, glob LRB} /\ N.c{1} = (LRB.l0{1} < LRB.l{1}) ? 1 : 0).
+      fun;wp.
+      if => //.
+        by call Eml;skip;progress => //; smt.
+      if => //.
+        inline{1} N(E, MR(E), B(A, ML(E), MR(E))).LRc.lr;wp.
+        by call Emr;wp;skip;progress => //;smt.
+      by call Emr;skip;progress => //; smt.
+      by conseq * Eleaks.
+      by conseq * Eenc.
+    swap{1} 2 2.
+    by call Einit;wp;rnd;wp;skip;progress => //;smt.
+  save.
+
+  axiom losslessA (E0 <: AEnc{A}) (LR <: LR{A}):
+      islossless LR.lr =>
+      islossless E0.leaks => islossless E0.enc => islossless A(E0, LR).run.
+  axiom losslessML (E0 <: AEnc{ML}):
+    islossless E0.leaks => islossless E0.enc => islossless ML(E0).lr.
+  axiom losslessMR (E0 <: AEnc{MR}):
+    islossless E0.leaks => islossless E0.enc => islossless MR(E0).lr.
+  axiom losslessL: islossless E.leaks.
+  axiom losslessE: islossless E.enc.
+
+  local lemma losslessMLE : islossless ML(E).lr.
+  proof strict.
+    apply (losslessML E);[apply losslessL | apply losslessE].
+  qed.
+
+  local lemma losslessMRE : islossless MR(E).lr.
+  proof strict.
+    apply (losslessMR E);[apply losslessL | apply losslessE].
+  qed.
+  
+  axiom q_pos : 0 < q.
+
+  local lemma WL0_NLA &m: 
+     Pr[W(L).work(0) @ &m : res] = Pr[N(E,L,A).main() @ &m : res /\ N.c <= q ].
+  proof strict.
+    equiv_deno (_ : ={glob A, glob ML, glob MR} /\ x{1}=0 ==> 
+                    res{1} = (res{2} /\ N.c{2} <= q)) => //.
+    fun.
+    call (_: q < N.c,
+             ={glob ML, glob MR, glob E} /\ LRB.l0{1} = 0 /\ LRB.l{1} = N.c{2} /\ 0 <= LRB.l{1},
+             LRB.l0{1} = 0 /\ q < LRB.l{1}).
+      by apply losslessA.
+
+      fun.
+      if{1}.
+        by wp;call Eml;wp;skip;progress => //;smt.
+      rcondt{1} 1.
+        by intros &m0;skip;smt.
+      by wp;call Eml;wp;skip;progress => //;smt.
+      intros &m2 _;fun.
+      rcondt 1; first by skip;smt.
+      by wp;call losslessMLE;skip;smt.
+      intros &m1;fun.
+      by call losslessMLE;wp;skip;smt.
+      
+      by conseq * Eleaks.
+      intros &m2 _;conseq * losslessL.
+      intros &m1; conseq * losslessL.
+
+      by conseq * Eenc.
+      intros &m2 _;conseq * losslessE.
+      intros &m1; conseq * losslessE.
+    
+    by call Einit;wp;skip;progress => //;smt.
+  qed.
+
+  local lemma WRq_NRA &m: 
+     Pr[W(R).work((q-1)) @ &m : res] = Pr[N(E,R,A).main() @ &m : res /\ N.c <= q ].
+  proof strict.
+    equiv_deno (_ : ={glob A, glob ML, glob MR} /\ x{1}=q-1 ==> 
+                    res{1} = (res{2} /\ N.c{2} <= q)) => //.
+    fun.
+    call (_: q < N.c,
+             ={glob ML, glob MR, glob E} /\ LRB.l0{1} = q-1 /\ LRB.l{1} = N.c{2} /\ 0 <= LRB.l{1},
+             LRB.l0{1} = q-1 /\ q < LRB.l{1}).
+      by apply losslessA.
+
+      fun.
+      if{1}.
+        by wp;call{1} losslessMLE;call{2} losslessMRE;wp;skip; smt.
+      if{1}.
+        by wp;call Emr;wp;skip;progress => //;smt.
+      by wp;call Emr;wp;skip;progress => //;smt.
+      intros &m2 _;fun.
+      rcondt 1; first by skip;smt.
+      by wp;call losslessMLE;skip; smt.
+      by intros &m1;fun;call losslessMRE;wp;skip;smt.
+      
+      by conseq * Eleaks.
+      intros &m2 _;conseq * losslessL.
+      intros &m1; conseq * losslessL.
+
+      by conseq * Eenc.
+      intros &m2 _;conseq * losslessE.
+      intros &m1; conseq * losslessE.
+    
+    by call Einit;wp;skip;progress => //;smt.
+  qed.
+
+  local lemma WLR_shift &m v: 1 <= v <= q-1 => 
+       Pr[W(L).work(v) @ &m: res] = Pr[W(R).work((v-1)) @ &m : res].
+  proof strict.
+    intros Hv;equiv_deno (_: ={glob A, glob ML, glob MR} /\ x{1} = v /\ x{2} = v-1 ==> ={res}) => //.
+    fun.
+    call (_: ={glob ML, glob MR, glob E, LRB.l} /\ LRB.l0{1} = v /\ LRB.l0{2} = v-1).
+      fun.
+      if{1}.        
+        rcondt{2} 1;first by intros &m0;skip;smt.
+        by wp;call Eml.
+      if{1}.
+        rcondt{2} 1;first by intros &m0;skip;smt.
+        by wp;call Eml.
+      rcondf{2} 1;first by intros &m0;skip;smt.
+      by if{2};wp;call Emr.
+      by conseq * Eleaks.
+      by conseq * Eenc.
+    by call Einit;wp.
+  qed.
+
+  (* TODO : move this *)
+  lemma Mrplus_inter_shift (i j k:int) f: 
+      Mrplus.sum f (Interval.interval i j) = 
+      Mrplus.sum (lambda l, f (l + k)) (Interval.interval (i-k) (j-k)).
+  proof strict.
+    rewrite (Mrplus.sum_chind f (lambda l, l - k) (lambda l, l + k)) /=;first smt.
+    congr => //.   
+    apply FSet.set_ext => x.
+    rewrite img_def Interval.mem_interval;split.
+      intros [y];rewrite Interval.mem_interval;smt.
+    intros Hx;exists (x+k);rewrite Interval.mem_interval;smt.
+  qed.
+
+  lemma Hybrid &m : 
+     Pr[N(E,ML(E),B(A,ML(E),MR(E))).main() @ &m : res /\ N.c <= 1] - 
+        Pr[N(E,MR(E),B(A,ML(E),MR(E))).main() @ &m : res /\ N.c <= 1] = 
+     1%r/q%r * (
+       Pr[N(E,ML(E),A).main() @ &m : res /\ N.c <= q] - 
+         Pr[N(E,MR(E),A).main() @ &m : res /\ N.c <= q]).
+  proof strict.
+    rewrite (NWL &m) (NWR &m) -(WL0_NLA &m) -(WRq_NRA &m).
+    cut Hint : Finite.(==) (create (support [0..q - 1])) (Interval.interval 0 (q - 1)).
+      by intros x;rewrite mem_create Interval.mem_interval /support Dinter.supp_def.
+    cut Hfin: Finite.finite (create (support [0..q - 1])).
+      by exists (Interval.interval 0 (q-1)).
+    cut Huni : forall (x : int), in_supp x [0..q - 1] => mu_x [0..q - 1] x = 1%r / q%r.
+      by intros x Hx;rewrite Dinter.mu_x_def_in //;smt.
+    cut := M.Mean_uni (W(L)) &m (lambda j g r, r) (1%r/q%r) _ _ => // /= ->.
+    cut := M.Mean_uni (W(R)) &m (lambda j g r, r) (1%r/q%r) _ _ => // /= ->.
+    cut -> : Finite.toFSet (create (support [0..q - 1])) = Interval.interval 0 (q-1).
+      apply FSet.set_ext => x.
+      by rewrite Interval.mem_interval Finite.mem_toFSet // mem_create /support Dinter.supp_def.
+    rewrite {1}Interval.interval_addl;first by smt.
+    rewrite (Interval.interval_pos 0 (q-1));first by smt.
+    rewrite Mrplus.sum_add /=.
+      by rewrite Interval.mem_interval.
+    rewrite Mrplus.sum_add /=.
+      by rewrite Interval.mem_interval;smt.
+    cut Hq : q%r <> Real.zero by smt.
+    fieldeq => //.
+    rewrite -(Mrplus.sum_comp (( * ) (-1)%r)) //;first intros x y;ringeq.
+    rewrite (Mrplus_inter_shift 0 (q - 1 - 1) (-1)) /=.
+    cut -> : q - 1 - 1 - -1 = q - 1; first by smt.
+    rewrite Mrplus.sum_add2.
+    rewrite (Mrplus.NatMul.sum_const 0%r) /Mrplus.NatMul.( * ) /=;last ringeq.
+    intros x; rewrite Interval.mem_interval => Hx;rewrite (WLR_shift &m x) //.
+      (* cut -> : x + -1 = x - 1     BUG *) 
+    by smt.
+  qed.
+
+  end section.
+
+end Hybrid.
